.dir-locals.el
@@ -1,1 +1,1 @@
-((coq-mode . ((coq-load-path . ("tlc" "flocq/src/Core" "flocq/src/Calc" "flocq/src/Prop" "flocq/src/Appli")))))
+((coq-mode . ((coq-load-path . ("coq" "tlc" "flocq/src/Core" "flocq/src/Calc" "flocq/src/Prop" "flocq/src/Appli")))))
